Small refactor of DupRegRem

src/NLustre/DupRegRem/DRR.v
@@ -1,67 +1,642 @@
+From Coq Require Import List.
+Import List.ListNotations.
+Open Scope list_scope.
+
+From Coq Require Import Recdef.
 From Velus Require Import Common.
+From Velus Require Import CommonProgram.
 From Velus Require Import Operators.
 From Velus Require Import Clocks.
-From Velus Require Import IndexedStreams.
-From Velus Require Import CommonTyping.
+From Velus Require Import Environment.
+From Velus Require Import CoreExpr.CESyntax.
+From Velus Require Import NLustre.NLSyntax.
 
-From Velus Require Import CoreExpr.CoreExpr.
-From Velus Require Export NLustre.NLSyntax.
-From Velus Require Export NLustre.IsDefined.
-From Velus Require Export NLustre.Memories.
-From Velus Require Export NLustre.NLIndexedSemantics.
-From Velus Require Export NLustre.NLOrdered.
-From Velus Require Export NLustre.NLClocking.
-From Velus Require Export NLustre.NLTyping.
-From Velus Require Export NLustre.NLNormalArgs.
-From Velus Require Export NLustre.DupRegRem.DupRegRem.
-From Velus Require Export NLustre.DupRegRem.DRRTyping.
-From Velus Require Export NLustre.DupRegRem.DRRClocking.
-From Velus Require Export NLustre.DupRegRem.DRRNormalArgs.
-From Velus Require Export NLustre.DupRegRem.DRRCorrectness.
+(** Remove duplicate registers in an NLustre program *)
 
 Module Type DRR
-       (Ids   : IDS)
-       (Op    : OPERATORS)
-       (OpAux : OPERATORS_AUX Ids Op)
-       (ComTyp: COMMONTYPING Ids Op OpAux)
-       (Cks   : CLOCKS Ids Op OpAux)
-       (IStr  : INDEXEDSTREAMS Ids Op OpAux Cks)
-       (CE    : COREEXPR Ids Op OpAux ComTyp Cks IStr)
-       (Syn   : NLSYNTAX Ids Op OpAux Cks CE.Syn)
-       (Ord   : NLORDERED Ids Op OpAux Cks CE.Syn Syn)
-       (Typ   : NLTYPING Ids Op OpAux Cks CE.Syn Syn Ord CE.Typ)
-       (Norm  : NLNORMALARGS Ids Op OpAux Cks CE.Syn CE.Typ Syn Ord Typ)
-       (Mem   : MEMORIES Ids Op OpAux Cks CE.Syn Syn)
-       (IsD   : ISDEFINED Ids Op OpAux Cks CE.Syn Syn Mem)
-       (Clo   : NLCLOCKING Ids Op OpAux Cks CE.Syn Syn Ord Mem IsD CE.Clo)
-       (Sem   : NLINDEXEDSEMANTICS Ids Op OpAux Cks CE.Syn Syn IStr Ord CE.Sem).
-  Declare Module Export DupRegRem  : DUPREGREM            Ids Op OpAux Cks CE.Syn Syn.
-  Declare Module Export DRRTyp     : DRRTYPING            Ids Op OpAux Cks CE.Syn CE.Typ Syn Ord Typ DupRegRem.
-  Declare Module Export DRRClo     : DRRCLOCKING          Ids Op OpAux Cks CE.Syn CE.Clo Syn Ord Mem IsD Clo DupRegRem.
-  Declare Module Export DRRNorm    : DRRNORMALARGS        Ids Op OpAux Cks CE.Syn CE.Typ Syn Ord Typ Norm DupRegRem.
-  Declare Module Export DRRCor     : DRRCORRECTNESS       Ids Op OpAux Cks IStr CE.Syn CE.Sem Syn Ord Sem DupRegRem.
+       (Import Ids   : IDS)
+       (Import Op    : OPERATORS)
+       (Import OpAux : OPERATORS_AUX   Ids Op)
+       (Import Cks   : CLOCKS      Ids Op OpAux)
+       (Import CESyn : CESYNTAX    Ids Op OpAux Cks)
+       (Import Syn   : NLSYNTAX    Ids Op OpAux Cks CESyn).
+
+  Definition const_dec : forall (c1 c2 : const),
+    { c1 = c2 } + { c1 <> c2 }.
+  Proof.
+    decide equality.
+    1-2:auto using cconst_dec, Nat.eq_dec.
+  Defined.
+
+  Definition exp_dec : forall (e1 e2 : exp),
+    { e1 = e2 } + { e1 <> e2 }.
+  Proof.
+    decide equality.
+    1-11:auto using cconst_dec, Nat.eq_dec, Pos.eq_dec.
+    1-3,5:apply EqDec_instance_5.
+    apply EqDec_instance_3.
+    apply EqDec_instance_4.
+  Defined.
+
+  Instance: EqDec const eq := { equiv_dec := const_dec }.
+  Instance: EqDec exp eq := { equiv_dec := exp_dec }.
+
+  Definition find_duplicates (eqs : list equation) : Env.t ident :=
+    snd (fold_left
+           (fun '(regs, sub) eq =>
+              match eq with
+              | EqFby x ck c0 e xr =>
+                let xr := PSP.of_list (List.map fst xr) in
+                match List.find
+                        (fun '(x, ck', c0', e', xr') =>
+                           (ck' ==b ck) && (c0' ==b c0) && (e' ==b e) && PS.equal xr' xr) regs
+                with
+                | Some (x', _, _, _ , _) => (regs, Env.add x x' sub)
+                | None => ((x, ck, c0, e, xr)::regs, sub)
+                end
+              | _ => (regs, sub)
+              end) eqs ([], Env.empty _)).
+
+  Section rename.
+    Variable (sub : Env.t ident).
+
+    Definition rename_in_var (x : ident) :=
+      match Env.find x sub with
+      | Some x' => x'
+      | None => x
+      end.
+
+    Fixpoint rename_in_clock (ck : clock) :=
+      match ck with
+      | Cbase => Cbase
+      | Con ck' x t => Con (rename_in_clock ck') (rename_in_var x) t
+      end.
+
+    Fixpoint rename_in_exp (e : exp) :=
+      match e with
+      | Econst _ | Eenum _ _ => e
+      | Evar x ty => Evar (rename_in_var x) ty
+      | Ewhen e x t => Ewhen (rename_in_exp e) (rename_in_var x) t
+      | Eunop op e1 ty => Eunop op (rename_in_exp e1) ty
+      | Ebinop op e1 e2 ty => Ebinop op (rename_in_exp e1) (rename_in_exp e2) ty
+      end.
+
+    Fixpoint rename_in_cexp (e : cexp) :=
+      match e with
+      | Emerge (x, te) ces ty =>
+        Emerge (rename_in_var x, te) (List.map rename_in_cexp ces) ty
+      | Ecase e ces d =>
+        Ecase (rename_in_exp e) (map (option_map rename_in_cexp) ces) (rename_in_cexp d)
+      | Eexp e => Eexp (rename_in_exp e)
+      end.
+
+    Definition rename_in_reset :=
+      map (fun '(xr, ckr) => (rename_in_var xr, rename_in_clock ckr)).
+
+    Definition rename_in_equation (equ : equation) :=
+      match equ with
+      | EqDef x ck ce => EqDef x (rename_in_clock ck) (rename_in_cexp ce)
+      | EqApp xs ck f es xr =>
+        EqApp xs (rename_in_clock ck) f (map rename_in_exp es) (rename_in_reset xr)
+      | EqFby x ck c0 e xr =>
+        EqFby x (rename_in_clock ck) c0 (rename_in_exp e) (rename_in_reset xr)
+      end.
+
+    Definition subst_and_filter_vars (vars : list (ident * (type * clock))) :=
+      let vars' := List.filter (fun '(x, _) => negb (Env.mem x sub)) vars in
+      List.map (fun '(x, (ty, ck)) => (x, (ty, rename_in_clock ck))) vars'.
+
+    Definition subst_and_filter_equations (eqs : list equation) :=
+      let eqs' := List.filter (fun eq => match eq with
+                                      | EqFby x _ _ _ _ => negb (Env.mem x sub)
+                                      | _ => true
+                                      end) eqs in
+      List.map rename_in_equation eqs'.
+
+  End rename.
+
+  Definition remove_dup_regs_eqs_once (vars : list (ident * (type * clock))) (eqs : list equation) :=
+    let sub' := find_duplicates eqs in
+    (subst_and_filter_vars sub' vars, subst_and_filter_equations sub' eqs).
+
+  Function remove_dup_regs_eqs (vars : list (ident * (type * clock))) (eqs : list equation) {measure length eqs} :=
+    let (vars', eqs') := remove_dup_regs_eqs_once vars eqs in
+    if (length eqs') <? (length eqs)
+    then remove_dup_regs_eqs vars' eqs'
+    else (vars, eqs).
+  Proof.
+    intros ????? Hlen.
+    apply Nat.ltb_lt in Hlen; auto.
+  Defined.
+
+  (** ** Properties *)
+
+  Lemma rename_in_exp_typeof : forall sub e,
+      typeof (rename_in_exp sub e) = typeof e.
+  Proof.
+    induction e; intros; simpl; auto.
+  Qed.
+
+  Lemma rename_in_cexp_typeofc : forall sub e,
+      typeofc (rename_in_cexp sub e) = typeofc e.
+  Proof.
+    induction e; intros; simpl; auto using rename_in_exp_typeof.
+    destruct p; auto.
+  Qed.
+
+  Lemma subst_and_filter_vars_InMembers : forall x sub vars,
+      InMembers x (subst_and_filter_vars sub vars) ->
+      InMembers x vars.
+  Proof.
+    induction vars as [|(?&?&?)]; intros Hin; simpl in *; auto.
+    unfold subst_and_filter_vars in Hin; simpl in Hin.
+    destruct (negb _); simpl; auto.
+    inv Hin; auto.
+  Qed.
+
+  Lemma subst_and_filter_vars_NoDupMembers : forall sub vars,
+      NoDupMembers vars ->
+      NoDupMembers (subst_and_filter_vars sub vars).
+  Proof.
+    induction vars as [|(?&?&?)]; intros Hnd; inv Hnd; simpl in *; auto.
+    - constructor.
+    - unfold subst_and_filter_vars; simpl.
+      destruct (negb _); simpl; auto.
+      constructor; auto.
+      contradict H1; eauto using subst_and_filter_vars_InMembers.
+  Qed.
+
+  Lemma remove_dup_regs_eqs_fby_incl : forall sub eqs,
+      incl (vars_defined (filter is_fby (snd (remove_dup_regs_eqs sub eqs))))
+           (vars_defined (filter is_fby eqs)).
+  Proof.
+    intros.
+    functional induction (remove_dup_regs_eqs sub eqs).
+    - etransitivity; eauto.
+      clear - e. inv e.
+      generalize (find_duplicates eqs) as sub'; intros.
+      induction eqs as [|[| |] ?]; simpl; auto using List.incl_refl.
+      unfold subst_and_filter_equations in *; simpl.
+      destruct (Env.mem i sub'); simpl; auto using incl_tl, incl_tl'.
+    - reflexivity.
+  Qed.
+
+  Lemma find_duplicates_spec : forall x y eqs,
+      Env.find x (find_duplicates eqs) = Some y ->
+      exists ck c e xr1 xr2,
+        In (EqFby x ck c e xr1) eqs /\
+        In (EqFby y ck c e xr2) eqs /\
+        PS.Equal (PSP.of_list (map fst xr1)) (PSP.of_list (map fst xr2)).
+  Proof.
+    unfold find_duplicates.
+    intros *.
+    setoid_rewrite (in_rev eqs).
+    rewrite <-fold_left_rev_right.
+    generalize (rev eqs); clear eqs; intros eqs.
+    remember (fold_right _ _ _) as find_duplicates.
+    assert ((forall x ck c0 e xr, In (x, ck, c0, e, xr) (fst find_duplicates) ->
+                          exists xr', In (EqFby x ck c0 e xr') eqs /\ PS.Equal (PSP.of_list (map fst xr')) xr) /\
+            (Env.find x (snd find_duplicates) = Some y ->
+             exists (ck : clock) (c : const) (e : exp) (xr1 xr2 : list (ident * clock)),
+               In (EqFby x ck c e xr1) eqs /\
+               In (EqFby y ck c e xr2) eqs /\ PS.Equal (PSP.of_list (map fst xr1)) (PSP.of_list (map fst xr2)))
+           ) as (?&?); auto.
+    subst.
+    induction eqs as [|[| |]]; intros *; (split; [intros * Hin|intros * Hfind]); simpl in *;
+      try destruct IHeqs as (IHeqs1&IHeqs2).
+    - inv Hin.
+    - rewrite Env.gempty in Hfind; congruence.
+    - destruct (fold_right _ _) eqn:Hfold.
+      eapply IHeqs1 in Hin as (?&?&?); eauto.
+    - destruct (fold_right _ _) eqn:Hfold.
+      eapply IHeqs2 in Hfind as (?&?&?&?&?&?&?&?); eauto 11.
+    - destruct (fold_right _ _) eqn:Hfold.
+      eapply IHeqs1 in Hin as (?&?&?); eauto.
+    - destruct (fold_right _ _) eqn:Hfold.
+      eapply IHeqs2 in Hfind as (?&?&?&?&?&?&?&?); eauto 11.
+    - destruct (fold_right _ _) eqn:Hfold.
+      destruct (find _ _) as [((((?&?)&?)&?)&?)|]; simpl in *.
+      2:destruct Hin as [Hin|Hin].
+      1,3:eapply IHeqs1 in Hin as (?&?&?); eauto.
+      inv Hin. do 1 eexists. split; eauto. reflexivity.
+    - destruct (fold_right _ _) eqn:Hfold.
+      destruct (find _ _) as [((((?&?)&?)&?)&?)|] eqn:Hfind'; simpl in *.
+      destruct (ident_eq_dec x i); subst.
+      2:rewrite Env.gso in Hfind; auto.
+      2,3:(eapply IHeqs2 in Hfind as (?&?&?&?&?&?&?&?); eauto 11).
+      rewrite Env.gss in Hfind; inv Hfind.
+      eapply find_some in Hfind' as (Hin&?).
+      eapply IHeqs1 in Hin as (?&Hin&Heq).
+      repeat rewrite Bool.andb_true_iff in H. destruct H as (((Heq1&Heq2)&Heq3)&Heq4).
+      rewrite equiv_decb_equiv in Heq1; inv Heq1.
+      rewrite equiv_decb_equiv in Heq2; inv Heq2.
+      rewrite equiv_decb_equiv in Heq3; inv Heq3.
+      apply PSF.equal_2 in Heq4.
+      do 7 (eexists; eauto).
+      symmetry. etransitivity; eauto.
+  Qed.
+
+  Corollary find_duplicates_In : forall x eqs,
+      Env.In x (find_duplicates eqs) ->
+      In x (vars_defined eqs).
+  Proof.
+    intros * Hin.
+    eapply Env.In_find in Hin as (?&Hfind).
+    eapply find_duplicates_spec in Hfind as (?&?&?&?&?&?&_).
+    eapply in_flat_map. do 2 (eexists; eauto). simpl; auto.
+  Qed.
+
+  Import Permutation.
+
+  Lemma find_duplicates_irrefl: forall x y eqs,
+      NoDup (vars_defined eqs) ->
+      Env.find x (find_duplicates eqs) = Some y ->
+      ~Env.In y (find_duplicates eqs).
+  Proof.
+    unfold find_duplicates.
+    intros * Hnd.
+    assert (NoDup (vars_defined (rev eqs))) as Hnd'.
+    { eapply Permutation_NoDup; [|eauto].
+      eapply Permutation_flat_map_Proper, Permutation_rev. }
+    clear Hnd. revert Hnd' y.
+    rewrite <-fold_left_rev_right.
+    generalize (rev eqs); clear eqs; intros eqs Hnd.
+    remember (fold_right _ _ _) as find_duplicates.
+    assert ((forall x ck c0 e xr, In (x, ck, c0, e, xr) (fst find_duplicates) -> ~Env.In x (snd find_duplicates) /\ In x (vars_defined eqs)) /\
+            (forall y, Env.find x (snd find_duplicates) = Some y ->
+                  ~ Env.In y (snd find_duplicates) /\
+                  In x (vars_defined eqs) /\ In y (vars_defined eqs))) as (_&?).
+    2:intros; apply H; auto.
+    revert x Hnd; subst.
+    induction eqs as [|[| |]]; intros x Hnd; (split; [intros * Hin|intros * Hfind]); simpl in *.
+    - inv Hin.
+    - rewrite Env.gempty in Hfind; congruence.
+    - inv Hnd. destruct (fold_right _ _) eqn:Hfold.
+      eapply IHeqs in Hin as (?&?); eauto.
+    - inv Hnd. destruct (fold_right _ _) eqn:Hfold.
+      apply IHeqs in Hfind as (?&?&?); auto.
+    - apply NoDup_app_r in Hnd.
+      destruct (fold_right _ _) eqn:Hfold.
+      rewrite in_app_iff.
+      eapply IHeqs in Hin as (?&?); eauto.
+    - apply NoDup_app_r in Hnd.
+      destruct (fold_right _ _) eqn:Hfold.
+      repeat rewrite in_app_iff.
+      apply IHeqs in Hfind as (?&?&?); auto.
+    - inv Hnd. destruct (fold_right _ _) eqn:Hfold.
+      destruct (find _ _) as [((((?&?)&?)&?)&?)|] eqn:Hfind'; simpl in *.
+      rewrite Env.Props.P.F.add_in_iff, not_or'; split.
+      3:destruct Hin as [?|Hin]. 3:inv H; split; auto.
+      1,2,4:eapply IHeqs in Hin as (?&?); eauto.
+      + split; auto.
+        intro contra; subst. congruence.
+      + intro contra. eapply Env.In_find in contra as (?&contra).
+        unfold Env.MapsTo in contra.
+        eapply IHeqs in contra as (?&?&?); eauto.
+    - inv Hnd. destruct (fold_right _ _) eqn:Hfold.
+      destruct (find _ _) as [((((?&?)&?)&?)&?)|] eqn:Hfind'; simpl in *.
+      destruct (ident_eq_dec x i); subst.
+      3:apply IHeqs in Hfind as (?&?&?); auto.
+      1,2:rewrite Env.Props.P.F.add_in_iff, not_or'.
+      + rewrite Env.gss in Hfind; inv Hfind.
+        eapply find_some in Hfind' as (Hin&_).
+        eapply IHeqs in Hin as (?&?); eauto. repeat split; auto.
+        intro contra; subst. congruence.
+      + rewrite Env.gso in Hfind; auto.
+        eapply IHeqs in Hfind as (?&?&?); eauto.
+        repeat split; auto.
+        intro; subst. congruence.
+  Qed.
+
+  Lemma subst_and_filter_equations_incl : forall sub eqs,
+      incl (vars_defined (subst_and_filter_equations sub eqs))
+           (vars_defined eqs).
+  Proof.
+    induction eqs as [|[| |]]; intros ? Hin; simpl in *; auto.
+    - inv Hin; auto.
+    - rewrite in_app_iff in *. inv Hin; auto.
+    - unfold subst_and_filter_equations in Hin; simpl in Hin.
+      destruct (negb _); simpl in *; auto. inv Hin; auto.
+  Qed.
+
+  Lemma subst_and_filter_equations_NoDup : forall sub eqs,
+      NoDup (vars_defined eqs) ->
+      NoDup (vars_defined (subst_and_filter_equations sub eqs)).
+  Proof.
+    induction eqs as [|[| |]]; intros Hnd; simpl in *; auto.
+    - inv Hnd. constructor; auto.
+      contradict H1. apply subst_and_filter_equations_incl in H1; auto.
+    - rewrite NoDup_app'_iff in *. destruct Hnd as (?&?&?).
+      repeat split; auto.
+      eapply Forall_impl; eauto. intros.
+      contradict H2.
+      apply subst_and_filter_equations_incl in H2; auto.
+    - inv Hnd.
+      unfold subst_and_filter_equations; simpl.
+      destruct (negb _); simpl; auto.
+      constructor; auto.
+      contradict H1.
+      apply subst_and_filter_equations_incl in H1; auto.
+  Qed.
+
+  (** *** vars_defined *)
+
+  Lemma find_duplicates_is_fby : forall x eqs,
+      NoDup (vars_defined eqs) ->
+      Env.In x (find_duplicates eqs) ->
+      forall eq, In eq eqs ->
+            In x (var_defined eq) ->
+            is_fby eq = true.
+  Proof.
+    unfold find_duplicates. intros * Hnd Henvin.
+    rewrite <-fold_left_rev_right in Henvin.
+    assert (NoDup (vars_defined (rev eqs))) as Hnd'.
+    { unfold vars_defined. rewrite <-Permutation_rev; auto. }
+    setoid_rewrite (in_rev eqs).
+    clear Hnd. revert Hnd' Henvin. generalize (rev eqs) as eqs'. clear eqs.
+    intros eqs.
+    induction eqs as [|[| |]]; intros * Hnd Hinsub ? Hineq Hin; simpl in *.
+    - exfalso. apply Env.Props.P.F.empty_in_iff in Hinsub; auto.
+    - destruct (fold_right _ _ _) eqn:Hfold.
+      inv Hnd. destruct Hineq; subst; simpl in *; auto.
+      destruct Hin; auto; subst.
+      exfalso. eapply H1.
+      { clear - Hfold Hinsub.
+        revert l t Hinsub Hfold.
+        induction eqs as [|[| |]]; intros; simpl in *.
+        - inv Hfold. apply Env.Props.P.F.empty_in_iff in Hinsub; auto.
+        - destruct (fold_right _ _ _) eqn:Hfold'; inv Hfold; eauto.
+        - destruct (fold_right _ _ _) eqn:Hfold'; inv Hfold; eauto.
+          apply in_or_app; eauto.
+        - destruct (fold_right _ _ _) eqn:Hfold'.
+          destruct (find _ _) as [((((?&?)&?)&?)&?)|]; inv Hfold; simpl in *; eauto.
+          apply Env.Props.P.F.add_in_iff in Hinsub as [?|Hinsub]; eauto.
+      }
+    - destruct (fold_right _ _ _) eqn:Hfold.
+      destruct Hineq; subst; simpl in *; eauto using NoDup_app_r.
+      eapply NoDup_app_In in Hnd; eauto.
+      exfalso. eapply Hnd.
+      { clear - Hfold Hinsub.
+        revert l2 t Hinsub Hfold.
+        induction eqs as [|[| |]]; intros; simpl in *.
+        - inv Hfold. apply Env.Props.P.F.empty_in_iff in Hinsub; auto.
+        - destruct (fold_right _ _ _) eqn:Hfold'; inv Hfold; eauto.
+        - destruct (fold_right _ _ _) eqn:Hfold'; inv Hfold; eauto.
+          apply in_or_app; eauto.
+        - destruct (fold_right _ _ _) eqn:Hfold'.
+          destruct (find _ _) as [((((?&?)&?)&?)&?)|]; inv Hfold; simpl in *; eauto.
+          apply Env.Props.P.F.add_in_iff in Hinsub as [?|Hinsub]; eauto.
+      }
+    - inv Hnd.
+      destruct (fold_right _ _ _) eqn:Hfold.
+      destruct (find _ _) as [((((?&?)&?)&?)&?)|]; simpl in *.
+      + apply Env.Props.P.F.add_in_iff in Hinsub as [?|Hinsub]; subst.
+        * destruct Hineq; subst; simpl in Hin; auto.
+          exfalso. apply H1.
+          unfold vars_defined. apply in_flat_map; eauto.
+        * destruct Hineq; subst; simpl in Hin; auto.
+      + destruct Hineq; subst; auto.
+  Qed.
+
+  Corollary find_duplicates_Forall_is_fby : forall eqs,
+      NoDup (vars_defined eqs) ->
+      Forall (fun eq => forall x, Env.In x (find_duplicates eqs) -> In x (var_defined eq) -> is_fby eq = true) eqs.
+  Proof.
+    intros.
+    eapply Forall_forall; intros.
+    eapply find_duplicates_is_fby; eauto.
+  Qed.
+
+  Lemma subst_and_filter_equations_vars_defined : forall sub eqs,
+      Forall (fun eq => forall x, Env.In x sub -> In x (var_defined eq) -> is_fby eq = true) eqs ->
+      vars_defined (subst_and_filter_equations sub eqs) =
+      filter (fun k => negb (Env.mem k sub)) (vars_defined eqs).
+  Proof.
+    induction eqs as [|[| |]]; intros Hf; inv Hf; simpl; auto.
+    2:rewrite <-filter_app.
+    1-3:rewrite <-IHeqs; eauto.
+    - destruct (Env.mem _ _) eqn:Hmem; simpl; auto.
+      exfalso. apply Env.mem_2, H1 in Hmem; simpl; auto.
+      inv Hmem.
+    - replace (filter (fun k => negb (Env.mem k sub)) l) with l; auto.
+      assert (Forall (fun x => ~Env.In x sub) l) as Hnin.
+      { clear - H1. apply Forall_forall; intros ?? contra.
+        apply H1 in contra; simpl in *; try congruence. }
+      clear -Hnin.
+      induction Hnin; simpl; auto.
+      apply Env.Props.P.F.not_mem_in_iff in H. rewrite H, <-IHHnin; auto.
+    - unfold subst_and_filter_equations; simpl.
+      destruct (negb _); simpl; auto.
+  Qed.
+
+  Lemma subst_and_filter_equations_Perm : forall sub eqs outs vars,
+      Forall (fun x => ~Env.In x sub) outs ->
+      Forall (fun eq => forall x, Env.In x sub -> In x (var_defined eq) -> is_fby eq = true) eqs ->
+      Permutation (vars_defined eqs) (map fst vars ++ outs) ->
+      Permutation (vars_defined (subst_and_filter_equations sub eqs))
+                  (map fst (subst_and_filter_vars sub vars) ++ outs).
+  Proof.
+    intros * Hnouts Hisfby.
+    unfold subst_and_filter_vars.
+    rewrite map_map; simpl. rewrite map_ext with (g:=fst) (l:=filter _ _).
+    2:(intros (?&?&?); auto).
+    replace (map fst (filter (fun '(k, _) => negb (Env.mem k sub)) vars))
+            with (filter (fun k => negb (Env.mem k sub)) (map fst vars)).
+    2:{ clear - vars. induction vars as [|(?&?)]; simpl; auto.
+        destruct (negb _); simpl; auto. f_equal; auto. }
+    generalize (map fst vars); clear vars; intros vars.
+    replace (filter (fun k => negb (Env.mem k sub)) vars ++ outs)
+      with (filter (fun k => negb (Env.mem k sub)) (vars ++ outs)).
+    2:{ rewrite <-filter_app. f_equal; auto.
+        induction Hnouts; simpl; auto.
+        apply Env.Props.P.F.not_mem_in_iff in H. rewrite H; simpl.
+        f_equal; auto. }
+    generalize (vars ++ outs); clear vars outs Hnouts.
+    intros. rewrite subst_and_filter_equations_vars_defined; auto.
+    rewrite H; auto.
+  Qed.
+
+  Lemma remove_dup_regs_eqs_Perm : forall vars eqs outs,
+      NoDup (vars_defined eqs) ->
+      Forall (fun x => ~In x (vars_defined (filter is_fby eqs))) outs ->
+      Permutation (vars_defined eqs) (map fst vars ++ outs) ->
+      Permutation (vars_defined (snd (remove_dup_regs_eqs vars eqs)))
+                  (map fst (fst (remove_dup_regs_eqs vars eqs)) ++ outs).
+  Proof.
+    intros *.
+    functional induction (remove_dup_regs_eqs vars eqs); simpl; intros * Hnd Houts Hperm; auto.
+    apply IHp; auto.
+    - inv e.
+      rewrite subst_and_filter_equations_vars_defined; auto using nodup_filter.
+      eapply find_duplicates_Forall_is_fby; eauto.
+    - eapply Forall_impl; eauto.
+      intros ??; simpl in *.
+      contradict H. clear - H e. inv e.
+      revert H. generalize (find_duplicates eqs). intros.
+      induction eqs as [|[| |]]; simpl in *; auto.
+      unfold subst_and_filter_equations in H; simpl in H.
+      destruct (Env.mem _ _); simpl in *; auto.
+      destruct H; auto.
+    - clear - Hnd Houts Hperm e. inv e.
+      apply subst_and_filter_equations_Perm; auto.
+      + eapply Forall_impl; eauto; intros; simpl in *.
+        intro contra.
+        assert (Hin:=contra). eapply find_duplicates_In in Hin.
+        eapply in_flat_map in Hin as (?&?&?).
+        eapply find_duplicates_is_fby in contra; eauto.
+        eapply H, in_flat_map. repeat esplit; eauto.
+        eapply filter_In; eauto.
+      + eapply find_duplicates_Forall_is_fby; eauto.
+  Qed.
+
+  Lemma remove_dup_regs_eqs_vars_InMembers : forall x vars eqs,
+      InMembers x (fst (remove_dup_regs_eqs vars eqs)) ->
+      InMembers x vars.
+  Proof.
+    intros *.
+    functional induction (remove_dup_regs_eqs vars eqs); intros; auto.
+    apply IHp in H; auto.
+    inv e. clear -H.
+    induction vars as [|(?&?&?)]; simpl in *; auto.
+    unfold subst_and_filter_vars in *; simpl in *.
+    destruct (negb _); auto.
+    inv H; simpl; auto.
+  Qed.
+
+  Lemma remove_dup_regs_eqs_vars_NoDupMembers : forall vars eqs,
+      NoDupMembers vars ->
+      NoDupMembers (fst (remove_dup_regs_eqs vars eqs)).
+  Proof.
+    intros *.
+    functional induction (remove_dup_regs_eqs vars eqs); intros; auto.
+    apply IHp.
+    inv e. clear -H.
+    induction vars as [|(?&?&?)]; inv H; simpl; try constructor.
+    unfold subst_and_filter_vars; simpl.
+    destruct (negb _); auto.
+    constructor; auto.
+    contradict H2. clear - H2.
+    induction vars as [|(?&?&?)]; simpl in *. inv H2.
+    destruct (negb _); auto.
+    inv H2; auto.
+  Qed.
+
+  (** ** Transformation of the node and global *)
+
+  Definition remove_dup_regs_eqs' vars eqs:
+    { res | remove_dup_regs_eqs vars eqs = res }.
+  Proof.
+    econstructor. reflexivity.
+  Defined.
+
+  Program Definition remove_dup_regs_node (n : node) : node :=
+    let res := remove_dup_regs_eqs' n.(n_vars) n.(n_eqs) in
+    {| n_name := n.(n_name);
+       n_in := n.(n_in);
+       n_out := n.(n_out);
+       n_vars := fst (proj1_sig res);
+       n_eqs := snd (proj1_sig res)
+    |}.
+  Next Obligation. exact n.(n_ingt0). Qed.
+  Next Obligation. exact n.(n_outgt0). Qed.
+  Next Obligation.
+    specialize (n_defd n) as Hdef.
+    specialize (n_vout n) as Hnout.
+    specialize (n_nodup n) as Hndup.
+    rewrite map_app.
+    apply remove_dup_regs_eqs_Perm; auto.
+    + apply NoDup_var_defined_n_eqs.
+    + apply Forall_forall; intros; eauto.
+    + rewrite <-map_app; auto.
+  Qed.
+  Next Obligation.
+    intro contra.
+    eapply n_vout; eauto.
+    eapply remove_dup_regs_eqs_fby_incl; eauto.
+  Qed.
+  Next Obligation.
+    specialize (n_nodup n) as Hnd.
+    repeat apply NoDupMembers_app.
+    - apply NoDupMembers_app_l in Hnd; auto.
+    - apply remove_dup_regs_eqs_vars_NoDupMembers; auto.
+      apply NoDupMembers_app_r, NoDupMembers_app_l in Hnd; auto.
+    - apply NoDupMembers_app_r, NoDupMembers_app_r in Hnd; auto.
+    - intros ? Hin.
+      intros Hout.
+      eapply NoDupMembers_app_r, NoDupMembers_app_InMembers in Hnd; eauto.
+      apply remove_dup_regs_eqs_vars_InMembers in Hin; auto.
+    - intros ? Hin.
+      eapply NoDupMembers_app_InMembers in Hnd; eauto.
+      rewrite InMembers_app in *.
+      contradict Hnd. destruct Hnd; auto.
+      left. apply remove_dup_regs_eqs_vars_InMembers in H; auto.
+  Qed.
+  Next Obligation.
+    specialize (n_good n) as Hgood.
+    repeat rewrite map_app, Forall_app in *.
+    destruct Hgood as ((Hin&Hvar&Hout)&Hname).
+    repeat (split; auto).
+    clear - Hvar.
+    eapply Forall_forall; intros.
+    apply fst_InMembers, remove_dup_regs_eqs_vars_InMembers, fst_InMembers in H.
+    eapply Forall_forall in Hvar; eauto.
+  Qed.
+
+  Local Program Instance remove_dup_regs_node_transform_unit: TransformUnit node node :=
+    { transform_unit := remove_dup_regs_node }.
+
+  Local Program Instance remove_dup_regs_without_units: TransformProgramWithoutUnits global global :=
+    { transform_program_without_units := fun g => Global g.(enums) [] }.
+
+  Definition remove_dup_regs : global -> global := transform_units.
+
+  (** *** Some properties *)
+
+  Lemma find_node_remove_dup_regs_forward : forall G f n,
+      find_node f G = Some n ->
+      find_node f (remove_dup_regs G) = Some (remove_dup_regs_node n).
+  Proof.
+    unfold remove_dup_regs, find_node.
+    intros * Hfind.
+    apply option_map_inv in Hfind as ((?&?)&Hfind&?); subst.
+    apply find_unit_transform_units_forward in Hfind.
+    rewrite Hfind; auto.
+  Qed.
+
+  Lemma find_node_remove_dup_regs_backward : forall G f n,
+      find_node f (remove_dup_regs G) = Some n ->
+      exists n0, find_node f G = Some n0 /\ n = remove_dup_regs_node n0.
+  Proof.
+    unfold remove_dup_regs, find_node.
+    intros * Hfind.
+    apply option_map_inv in Hfind as ((?&?)&Hfind&?); subst.
+    apply find_unit_transform_units_backward in Hfind as (?&?&Hfind&?&?); subst.
+    exists x. repeat split; auto.
+    rewrite Hfind; auto.
+  Qed.
+
+  Lemma remove_dup_regs_iface_eq : forall G,
+      global_iface_eq G (remove_dup_regs G).
+  Proof.
+    intros. split; intros; auto.
+    destruct (find_node _ _) eqn:Hfind.
+    - erewrite find_node_remove_dup_regs_forward; eauto.
+      constructor; simpl.
+      repeat (split; auto).
+    - destruct (find_node f (remove_dup_regs _)) eqn:Hfind'; try constructor.
+      exfalso.
+      apply find_node_remove_dup_regs_backward in Hfind' as (?&?&_); congruence.
+  Qed.
+
 End DRR.
 
 Module DRRFun
        (Ids   : IDS)
        (Op    : OPERATORS)
-       (OpAux : OPERATORS_AUX Ids Op)
-       (ComTyp: COMMONTYPING Ids Op OpAux)
-       (Cks   : CLOCKS Ids Op OpAux)
-       (IStr  : INDEXEDSTREAMS Ids Op OpAux Cks)
-       (CE    : COREEXPR Ids Op OpAux ComTyp Cks IStr)
-       (Syn   : NLSYNTAX Ids Op OpAux Cks CE.Syn)
-       (Ord   : NLORDERED Ids Op OpAux Cks CE.Syn Syn)
-       (Typ   : NLTYPING Ids Op OpAux Cks CE.Syn Syn Ord CE.Typ)
-       (Norm  : NLNORMALARGS Ids Op OpAux Cks CE.Syn CE.Typ Syn Ord Typ)
-       (Mem   : MEMORIES Ids Op OpAux Cks CE.Syn Syn)
-       (IsD   : ISDEFINED Ids Op OpAux Cks CE.Syn Syn Mem)
-       (Clo   : NLCLOCKING Ids Op OpAux Cks CE.Syn Syn Ord Mem IsD CE.Clo)
-       (Sem   : NLINDEXEDSEMANTICS Ids Op OpAux Cks CE.Syn Syn IStr Ord CE.Sem)
-       <: DRR Ids Op OpAux ComTyp Cks IStr CE Syn Ord Typ Norm Mem IsD Clo Sem.
-  Module Export DupRegRem  := DupRegRemFun            Ids Op OpAux Cks CE.Syn Syn.
-  Module Export DRRTyp     := DrrTypingFun            Ids Op OpAux Cks CE.Syn CE.Typ Syn Ord Typ DupRegRem.
-  Module Export DRRClo     := DrrClockingFun          Ids Op OpAux Cks CE.Syn CE.Clo Syn Ord Mem IsD Clo DupRegRem.
-  Module Export DRRNorm    := DrrNormalArgsFun        Ids Op OpAux Cks CE.Syn CE.Typ Syn Ord Typ Norm DupRegRem.
-  Module Export DRRCor     := DrrCorrectnessFun       Ids Op OpAux Cks IStr CE.Syn CE.Sem Syn Ord Sem DupRegRem.
+       (OpAux : OPERATORS_AUX   Ids Op)
+       (Cks   : CLOCKS      Ids Op OpAux)
+       (CESyn : CESYNTAX    Ids Op OpAux Cks)
+       (Syn   : NLSYNTAX    Ids Op OpAux Cks CESyn)
+<: DRR Ids Op OpAux Cks CESyn Syn.
+  Include DRR Ids Op OpAux Cks CESyn Syn.
 End DRRFun.
